% !TEX root = ../thesis.tex
\begin{figure}[h]
  \begin{center}
    \begin{tabular}{|l c l|}
      \hline
      \textsf{MonoidFlat} $:$ \textsf{LF} & &\\\hline
      $G$ & $:$ & $ \typett$\\
      $\circ$ & $:$ & $ G \rightarrow G \rightarrow G$\\
      $\plaintt{assoc}$& $:$ & $ \plaintt{ded}\left( \forall x \in G . \forall y \in G . \forall z \in G . (x\circ y)\circ z=x\circ (y\circ z) \right)$\\
      $e$ & $:$ & $G$\\
      $\plaintt{ident}$& $:$ & $ \plaintt{ded}\left( \forall x \in G x\circ e = e\circ x = x \right) $\\
      \hline
    \end{tabular}
  \end{center}

  \caption[A flattened Theory of Monoids]{
    An elaborated, flattened version of the Monoid theory from Figure~\ref{fig:theorygraph}. 
  }
  \label{fig:flattheory}
\end{figure}
